kalloc/Spec_kalloc.v
@@ -107,18 +107,23 @@ Definition kfree_spec (K:KallocFreeAPD) {cs: compspecs} (t: type) :=
           if eq_dec new_head nullval then 
           ASI_kalloc.mem_mgr K gv sh ls xx original_freelist_pointer
           else 
-          ASI_kalloc.mem_mgr K gv sh (original_freelist_pointer::ls) xx new_head
+          ASI_kalloc.mem_mgr K gv sh (original_freelist_pointer::ls) xx new_head *
+          memory_block sh (PGSIZE - (t_run_size)) (offset_val (t_run_size) new_head) (* not the whole block is used *)
             ).
 
 Definition kalloc_spec (K:KallocFreeAPD) {cs: compspecs} (t: type) :=
 DECLARE _kalloc
 WITH gv:globals, sh:share, ls: list val, xx:Z, original_freelist_pointer:val
 PRE [ ]
-    PROP(   (sizeof t) <= PGSIZE;
+    PROP(0 < (sizeof t) <= PGSIZE;
             complete_legal_cosu_type t = true;
             natural_aligned natural_alignment t = true) 
     PARAMS () GLOBALS(gv)
-    SEP ( ASI_kalloc.mem_mgr K gv sh ls xx original_freelist_pointer )  
+    SEP ( ASI_kalloc.mem_mgr K gv sh ls xx original_freelist_pointer *
+          if eq_dec original_freelist_pointer nullval then emp else
+          (
+     !! malloc_compatible (sizeof t) original_freelist_pointer &&
+    memory_block sh (PGSIZE - (t_run_size)) (offset_val (t_run_size) original_freelist_pointer)) )
 POST [ tptr tvoid ]
     PROP()
     RETURN (original_freelist_pointer) 
@@ -129,7 +134,8 @@ POST [ tptr tvoid ]
         (
           EX next ls',
           (!! (next :: ls' = ls) &&
-              type_kalloc_token K sh t original_freelist_pointer *
+              type_kalloc_token K sh t original_freelist_pointer * (*
+              memory_block sh (PGSIZE - (sizeof t)) (offset_val (sizeof t) original_freelist_pointer) *)
               ASI_kalloc.mem_mgr K gv sh ls' xx next
         )
         )
