kalloc/Verif_allocation_examples.v
@@ -16,7 +16,13 @@ Definition kalloc_write_42_spec : ident * funspec :=
     DECLARE _kalloc_write_42
     WITH sh : share, original_freelist_pointer:val, xx:Z, ls:list val, gv:globals
     PRE [ ] 
-        PROP () PARAMS() GLOBALS(gv) SEP (KAF_globals gv sh ls xx original_freelist_pointer)
+        PROP () PARAMS() GLOBALS(gv) 
+        SEP (KAF_globals gv sh ls xx original_freelist_pointer *
+            if eq_dec original_freelist_pointer nullval then emp else
+            (
+            !! malloc_compatible (sizeof (tint)) original_freelist_pointer &&
+            memory_block sh (PGSIZE - (t_run_size)) (offset_val (t_run_size) original_freelist_pointer))
+            )
     POST [ tint ] 
         EX r,
         PROP ( ) RETURN (r) SEP (
@@ -29,6 +35,8 @@ Definition kalloc_write_42_spec : ident * funspec :=
                     r = Vint (Int.repr 42)
                  ) &&
                     data_at sh tint (Vint (Int.repr 42)) original_freelist_pointer *
+                    memory_block sh (PGSIZE - sizeof tint)
+                        (offset_val (sizeof tint) original_freelist_pointer) *
                     KAF_globals gv  sh ls' xx next
             )
             )
@@ -38,9 +46,13 @@ Definition kalloc_int_array_spec : ident * funspec :=
     DECLARE _kalloc_int_array
     WITH sh : share, original_freelist_pointer:val, xx:Z, ls:list val, gv:globals, n:Z
     PRE [ tint ] 
-    PROP (0 <= n /\ sizeof (tarray tint n) <= PGSIZE) (* make sure an array of size n fits into the page *)
+    PROP (0 < n /\ 0 < sizeof (tarray tint n) /\ sizeof (tarray tint n) <= PGSIZE) (* make sure an array of size n fits into the page *)
     PARAMS(Vint (Int.repr n)) GLOBALS(gv) 
-    SEP (KAF_globals gv sh ls xx original_freelist_pointer)
+    SEP (KAF_globals gv sh ls xx original_freelist_pointer *
+    if eq_dec original_freelist_pointer nullval then emp else
+    (
+    !! malloc_compatible (sizeof (tarray tint n)) original_freelist_pointer &&
+    memory_block sh (PGSIZE - (t_run_size)) (offset_val (t_run_size) original_freelist_pointer)))
     POST [ tptr tint ]
     PROP ( ) RETURN () SEP (
         (if eq_dec original_freelist_pointer nullval then
@@ -49,6 +61,8 @@ Definition kalloc_int_array_spec : ident * funspec :=
         EX next ls',
             (!! (next :: ls' = ls) &&
                 array_42_rep sh n original_freelist_pointer *
+                memory_block sh (PGSIZE - sizeof (tarray tint n))
+                        (offset_val (sizeof (tarray tint n)) original_freelist_pointer) *
                 KAF_globals gv  sh ls' xx next
         )
         )
@@ -58,7 +72,12 @@ Definition kalloc_write_pipe_spec : ident * funspec :=
     DECLARE _kalloc_write_pipe
     WITH sh : share, original_freelist_pointer:val, xx:Z, ls:list val, gv:globals
     PRE [ ] 
-        PROP () PARAMS() GLOBALS(gv) SEP (KAF_globals gv sh ls xx original_freelist_pointer)
+        PROP () PARAMS() GLOBALS(gv) SEP (KAF_globals gv sh ls xx original_freelist_pointer
+        *
+        if eq_dec original_freelist_pointer nullval then emp else
+        (
+        !! malloc_compatible (sizeof t_struct_pipe) original_freelist_pointer &&
+        memory_block sh (PGSIZE - (t_run_size)) (offset_val (t_run_size) original_freelist_pointer)))
     POST [ tvoid ]
         PROP ( ) RETURN () SEP (
             (if eq_dec original_freelist_pointer nullval then
@@ -67,6 +86,8 @@ Definition kalloc_write_pipe_spec : ident * funspec :=
             EX next ls',
                 (!! (next :: ls' = ls) &&
                     pipe_rep sh original_freelist_pointer *
+                    memory_block sh (PGSIZE - sizeof (t_struct_pipe))
+                    (offset_val (sizeof (t_struct_pipe)) original_freelist_pointer) *
                     KAF_globals gv  sh ls' xx next
             )
             )
@@ -77,7 +98,12 @@ Definition kalloc_int_array_spec_fail : ident * funspec :=
     DECLARE _kalloc_int_array
     WITH sh : share, original_freelist_pointer:val, xx:Z, ls:list val, gv:globals, n:Z
     PRE [ tint ] 
-    PROP (0 <= n <= Int.max_signed) PARAMS(Vint (Int.repr n)) GLOBALS(gv) SEP (KAF_globals gv sh ls xx original_freelist_pointer)
+    PROP (0 < n <= Int.max_signed) PARAMS(Vint (Int.repr n)) GLOBALS(gv) 
+    SEP (KAF_globals gv sh ls xx original_freelist_pointer *
+    if eq_dec original_freelist_pointer nullval then emp else
+    (
+    !! malloc_compatible (sizeof (tarray tint n)) original_freelist_pointer &&
+    memory_block sh (PGSIZE - (t_run_size)) (offset_val (t_run_size) original_freelist_pointer)))
     POST [ tptr tint ]
     PROP ( ) RETURN () SEP (
         (if eq_dec original_freelist_pointer nullval then
@@ -86,6 +112,8 @@ Definition kalloc_int_array_spec_fail : ident * funspec :=
         EX next ls',
             (!! (next :: ls' = ls) &&
                 array_42_rep sh n original_freelist_pointer*
+                memory_block sh (PGSIZE - sizeof (tarray tint n))
+                        (offset_val (sizeof (tarray tint n)) original_freelist_pointer) *
                 KAF_globals gv  sh ls' xx next
         )
         )
@@ -94,39 +122,57 @@ Definition kalloc_int_array_spec_fail : ident * funspec :=
 Lemma body_kalloc_write_42: semax_body KAFVprog KAFGprog f_kalloc_write_42 kalloc_write_42_spec.
 Proof.
 start_function.
-forward. 
-forward_call (kalloc_spec_sub KAF_APD tint) (gv, sh , ls, xx, original_freelist_pointer ). (* kalloc *)
-- unfold KAF_globals. entailer!.
-- if_tac.
-    + forward_if.
-        * rewrite H in H0; auto_contradict.
-        * forward. Exists (Vint(Int.repr 0)). entailer.
-    + Intros ab.
+Intros.
+forward. if_tac_auto_contradict. 
+- forward_call (kalloc_spec_sub KAF_APD tint) (gv, sh , ls, xx, original_freelist_pointer ). (* kalloc *)
++ unfold KAF_globals. entailer!.
++ if_tac_auto_contradict.
+    * forward_if.
+        -- rewrite H in H1; auto_contradict.
+        -- forward. Exists (Vint(Int.repr 0)). entailer.
+- forward_call (kalloc_spec_sub KAF_APD tint) (gv, sh , ls, xx, original_freelist_pointer ). (* kalloc *)
+    + unfold KAF_globals. if_tac_auto_contradict. entailer!.
+    + if_tac_auto_contradict.
+    Intros ab.
       destruct ls; auto_contradict.
       forward_if.
         * unfold type_kalloc_token. rewrite kalloc_token_sz_split. Intros.
-        rewrite memory_block_data_at_; auto. rewrite data_at__eq. forward.
-        forward. forward.
+        assert (sizeof tint + (PGSIZE - sizeof tint) = PGSIZE). { try rep_lia. }
+        rewrite <- H11.
+        destruct original_freelist_pointer; auto_contradict.
+        assert (i = Ptrofs.repr (Ptrofs.unsigned i)). { rewrite Ptrofs.repr_unsigned. auto. }
+        rewrite H12.
+        rewrite memory_block_split with (m:=(PGSIZE - sizeof tint)); try rep_lia.
+        rewrite memory_block_data_at_; auto. rewrite data_at__eq. Intros.
+        forward. forward. forward.
         Exists (Vint(Int.repr 42)) (fst ab) (snd ab). entailer.
+        unfold KAF_globals. entailer!.
+        rewrite H12. entailer!.
+        rewrite <- H12. auto.
         * forward.
 Qed.
+
+
 
 Lemma body_kalloc_int_array: semax_body KAFVprog KAFGprog f_kalloc_int_array kalloc_int_array_spec.
 Proof.
 start_function.
-forward.
-forward_call (kalloc_spec_sub KAF_APD (tarray tint n)) (gv, sh , ls, xx, original_freelist_pointer ). (* kalloc *)
-- unfold KAF_globals. entailer!.
-(*- destruct H; auto.*)
-- if_tac.
-    + forward_if.
-        * rewrite H0 in H1; auto_contradict.
-        * forward. 
-    + Intros ab.
+Intros.
+forward. if_tac_auto_contradict; destruct H as [HH1 HH2].
+- forward_call (kalloc_spec_sub KAF_APD (tarray tint n)) (gv, sh , ls, xx, original_freelist_pointer ). (* kalloc *)
++ unfold KAF_globals. entailer!.
++ if_tac_auto_contradict.
+    * forward_if.
+        -- rewrite H in H1; auto_contradict.
+        -- forward.
+- forward_call (kalloc_spec_sub KAF_APD (tarray tint n)) (gv, sh , ls, xx, original_freelist_pointer ). (* kalloc *)
+    + unfold KAF_globals. if_tac_auto_contradict. entailer!.
+    + if_tac_auto_contradict.
+    Intros ab.
       destruct ls; auto_contradict.
       forward_if.
         * unfold type_kalloc_token. rewrite kalloc_token_sz_split. Intros.
-        rewrite memory_block_data_at_; auto. rewrite data_at__eq.
+        assert (sizeof (tarray tint n) + (PGSIZE - sizeof (tarray tint n)) = PGSIZE). { try rep_lia. }
         forward_for_simple_bound n
         (EX i:Z,
         PROP  ()
@@ -137,19 +183,37 @@ forward_call (kalloc_spec_sub KAF_APD (tarray tint n)) (gv, sh , ls, xx, origina
         SEP (
             (
                 tmp_array_42_rep sh n original_freelist_pointer i*
+                memory_block sh (PGSIZE - sizeof (tarray tint n))
+                        (offset_val (sizeof (tarray tint n)) original_freelist_pointer) *
                 KAF_globals gv sh ls xx v
             )
             )
         )%assert.
-        -- destruct H. unfold tarray in H7. rewrite sizeof_Tarray in H7. 
+        -- destruct HH2 as [HH2 HH3]. unfold tarray in HH3. rewrite sizeof_Tarray in HH3. 
         assert (Z.max 0 n <= PGSIZE / (sizeof tint)). {  apply Zdiv_le_lower_bound. simpl; try rep_lia. auto. rewrite Z.mul_comm. auto. }
         assert (n <= PGSIZE / (sizeof tint)); try rep_lia. apply (Z.le_trans) with (PGSIZE / sizeof tint). try rep_lia.
         unfold PGSIZE; simpl; try rep_lia.
-        -- entailer!. unfold tmp_array_42_rep. unfold KAF_globals. entailer!. inversion H1; entailer.
+        -- entailer. unfold tmp_array_42_rep. unfold KAF_globals. entailer. inversion H1; entailer.
+        destruct original_freelist_pointer; auto_contradict.
+        assert (i = Ptrofs.repr (Ptrofs.unsigned i)). { rewrite Ptrofs.repr_unsigned. auto. }
+        assert (Zrepeat (default_val tint) n = default_val (tarray tint n)) as Hdefault. {
+            apply Zrepeat_default_val_array. auto.
+        }
+        rewrite H12 at 1.
+        rewrite <- H10 at 1.
+        rewrite memory_block_split with (m:=(PGSIZE - sizeof (tarray tint n))); try rep_lia.
+        rewrite memory_block_data_at_; auto. rewrite data_at__eq. 
+        entailer!. simpl. entailer!.
+        rewrite <- H12.
+        rewrite H12.
+        rewrite Hdefault.
+        entailer!. 
+        rewrite Ptrofs.repr_unsigned. auto.
         -- Intros.
         assert (Int.min_signed <= i <= Int.max_signed). { 
             assert (n <= Int.max_signed). {
-            destruct H. unfold tarray in H7. unfold tarray in H8. rewrite sizeof_Tarray in H8. 
+            destruct HH2 as [HH2 HH3]. 
+            unfold tarray in HH3. unfold tarray in HH3. rewrite sizeof_Tarray in HH3. 
             assert (Z.max 0 n <= PGSIZE / (sizeof tint)). {  apply Zdiv_le_lower_bound. simpl; try rep_lia. auto. rewrite Z.mul_comm. auto. }
             assert (n <= PGSIZE / (sizeof tint)); try rep_lia. apply (Z.le_trans) with (PGSIZE / sizeof tint). try rep_lia.
             unfold PGSIZE; simpl; try rep_lia.
@@ -162,8 +226,8 @@ forward_call (kalloc_spec_sub KAF_APD (tarray tint n)) (gv, sh , ls, xx, origina
         ++ rewrite sublist_firstn. 
         rewrite firstn_app1.
         assert (Zlength (array_42 (Z.to_nat i)) = i). { rewrite array_42_length. try rep_lia. }
-        rewrite Zlength_length in H13; try rep_lia.
-        rewrite <- H13 at 1.
+        rewrite Zlength_length in H21; try rep_lia.
+        rewrite <- H21 at 1.
         rewrite firstn_exact_length with (xs :=array_42 (Z.to_nat i)); try rep_lia.
         rewrite sublist_app2.
         rewrite array_42_length.
@@ -184,7 +248,7 @@ forward_call (kalloc_spec_sub KAF_APD (tarray tint n)) (gv, sh , ls, xx, origina
             rewrite array_42_length.
             try rep_lia.
         }
-        rewrite H13; auto.
+        rewrite H21; auto.
         ++ rewrite Zlength_app. rewrite array_42_length. rewrite Zlength_Zrepeat; try rep_lia.
         -- forward. Exists v ls. entailer!. unfold tmp_array_42_rep. unfold array_42_rep. 
         replace (n - n) with 0; try rep_lia. 
@@ -194,10 +258,12 @@ Qed.
 
 Lemma body_kalloc_int_array_fail: semax_body KAFVprog KAFGprog f_kalloc_int_array kalloc_int_array_spec_fail.
 Proof.
-start_function.
+start_function. Intros.
 forward.
 forward_call (kalloc_spec_sub KAF_APD (tarray tint n)) (gv, sh , ls, xx, original_freelist_pointer ). (* kalloc *)
-- unfold KAF_globals. entailer!.
+- unfold KAF_globals. if_tac.
++ entailer!.
++ entailer!.
 - assert (exists n : Z, sizeof (tarray tint n) > PGSIZE). 
     {
         exists PGSIZE.
@@ -209,6 +275,7 @@ Abort.
 Lemma body_kalloc_write_pipe: semax_body KAFVprog KAFGprog f_kalloc_write_pipe kalloc_write_pipe_spec.
 Proof.
 start_function.
+Intros.
 forward.
 forward_call (kalloc_spec_sub KAF_APD t_struct_pipe) (gv, sh , ls, xx, original_freelist_pointer ). (* kalloc *)
 - unfold KAF_globals. entailer!. 
@@ -217,13 +284,28 @@ forward_call (kalloc_spec_sub KAF_APD t_struct_pipe) (gv, sh , ls, xx, original_
         * rewrite H in H0; auto_contradict.
         * forward. entailer.
     + Intros ab. forward_if.
+        *
         rewrite mem_mgr_split. rewrite type_kalloc_token_split. Intros. rewrite kalloc_token_sz_split.
-        Intros. 
-        rewrite memory_block_data_at_; auto. rewrite data_at__eq. Intros. forward.
-        forward. forward. forward. 
+        Intros.
+        assert (sizeof (t_struct_pipe) + (PGSIZE - sizeof (t_struct_pipe)) = PGSIZE) as HH12. { try rep_lia. }
+        rewrite <- HH12.
+        destruct original_freelist_pointer; auto_contradict.
+        assert (i = Ptrofs.repr (Ptrofs.unsigned i)) as HHH12. { rewrite Ptrofs.repr_unsigned. auto. }
+        rewrite HHH12.
+        rewrite memory_block_split with (m:=(PGSIZE - sizeof t_struct_pipe)); try rep_lia.
+        rewrite memory_block_data_at_; auto. rewrite data_at__eq. Intros.
+        forward. forward. forward. forward.
         entailer.
         Exists  (fst ab) (snd ab). entailer.
         unfold KAF_globals. unfold pipe_rep.  Exists (fst (default_val t_struct_pipe)). entailer!.
-        rewrite mem_mgr_split. entailer.
-        * forward. entailer.
+        rewrite mem_mgr_split. 
+        assert (i = Ptrofs.repr (Ptrofs.unsigned i)) as HH0. { rewrite Ptrofs.repr_unsigned. auto. }
+        rewrite <- HH0.
+        entailer!.
+        assert (i = Ptrofs.repr (Ptrofs.unsigned i)) as HH0. { rewrite Ptrofs.repr_unsigned. auto. }
+        rewrite <- HH0.
+        auto. try simpl; rep_lia.
+        try simpl; rep_lia.
+        * forward.
+        entailer!.
 Qed.
