kalloc/Verif_kalloc_kfree.v
@@ -11,7 +11,7 @@ Require Import VC.Spec_kalloc.
 
 Local Open Scope logic.
 
-Lemma body_kfree: semax_body KAFVprog KAFGprog f_kfree (kfree_spec KAF_APD t_run).
+(*Lemma body_kfree: semax_body KAFVprog KAFGprog f_kfree (kfree_spec KAF_APD t_run).
 Proof. start_function. Intros.
 forward.
 rewrite mem_mgr_split. Intros.
@@ -25,9 +25,136 @@ destruct (eq_dec new_head nullval).
      entailer. rewrite mem_mgr_split. refold_freelistrep. entailer!.
      right; split; auto. unfold not; auto_contradict.
     * forward. entailer.
+Qed.*)
+
+
+Lemma body_kfree': semax_body KAFVprog KAFGprog f_kfree (kfree_spec' KAF_APD _kfree).
+Proof. start_function.
+forward.
+rewrite mem_mgr_split. Intros.
+destruct (eq_dec new_head nullval).
+- forward_if.
+    * rewrite e in H2; auto_contradict.
+    * forward. entailer. rewrite mem_mgr_split. entailer.
+- forward_if.
+    * forward. rewrite kalloc_token_sz_split. Intros. 
+    assert (memory_block sh ((sizeof t_run) + (PGSIZE-sizeof t_run)) new_head = memory_block sh PGSIZE new_head).
+    {
+        simpl. unfold PGSIZE. auto.
+    }
+    rewrite <- H9.
+    destruct new_head; auto_contradict.
+    assert (memory_block sh ((sizeof t_run) + (PGSIZE - sizeof t_run)) (Vptr b i) = memory_block sh ((sizeof t_run) + (PGSIZE - sizeof t_run)) (Vptr b (Ptrofs.repr (Ptrofs.unsigned i)))). {
+        simpl. rewrite Ptrofs.repr_unsigned. auto.
+    }
+    rewrite H10.
+    rewrite memory_block_split; try rep_lia.
+    assert (Vptr b (Ptrofs.repr (Ptrofs.unsigned i)) = Vptr b (i)). { rewrite Ptrofs.repr_unsigned. auto. }
+    rewrite memory_block_data_at_.
+    Intros.
+    rewrite data_at__eq. rewrite H11. forward. forward. 
+    entailer. rewrite mem_mgr_split. refold_freelistrep. entailer!.
+    right; split; auto. unfold not; auto_contradict. 
+    unfold t_run_size. unfold offset_val. rewrite Ptrofs.add_unsigned. rewrite Ptrofs.unsigned_repr.
+    entailer!. simpl. try rep_lia. rewrite H11. auto.
+    * forward. entailer.
 Qed.
 
-Lemma body_kalloc: semax_body KAFVprog KAFGprog f_kalloc (kalloc_spec (KAF_APD) t_run).
+
+Lemma body_kalloc: semax_body KAFVprog KAFGprog f_kalloc (kalloc_spec' (KAF_APD) _kalloc).
+Proof. start_function.
+rewrite mem_mgr_split. Intros. forward. 
+if_tac.
+-
+forward_if (
+    PROP  ( )
+    LOCAL (
+        temp _r original_freelist_pointer; 
+        gvars gv
+        )
+    SEP (
+        if (eq_dec original_freelist_pointer nullval) then
+        (ASI_kalloc.mem_mgr KAF_APD gv sh ls xx original_freelist_pointer * emp)
+      else 
+        (
+          EX next ls',
+          (!! (next :: ls' = ls) &&
+              kalloc_token' KAF_APD sh n original_freelist_pointer *
+              ASI_kalloc.mem_mgr KAF_APD gv sh ls' xx next
+          )
+        )
+    )
+)%assert.
++ rewrite H2 in H3. auto_contradict.
++ forward. if_tac; auto_contradict. entailer!.
+    rewrite mem_mgr_split. entailer!.
++ if_tac_auto_contradict. forward.
+-
+forward_if (
+    PROP  ( )
+    LOCAL (
+        temp _r original_freelist_pointer; 
+        gvars gv
+        )
+    SEP (
+        if (eq_dec original_freelist_pointer nullval) then
+        (ASI_kalloc.mem_mgr KAF_APD gv sh ls xx original_freelist_pointer * emp)
+      else 
+        (
+          EX next ls',
+          (!! (next :: ls' = ls) &&
+              kalloc_token' KAF_APD sh n original_freelist_pointer *
+              ASI_kalloc.mem_mgr KAF_APD gv sh ls' xx next
+          )
+        )
+    )
+)%assert.
+
++destruct H1 as [[H0011 H0012] | [H0021 H0022]].
+    * rewrite H0012 in H3; auto_contradict.
+    * destruct ls; auto_contradict.
+    refold_freelistrep. Intros.
+    forward. forward.
+    entailer.
+    rewrite mem_mgr_split. Intros. 
+    refold_freelistrep. if_tac.
+    -- rewrite H14 in H0022; auto_contradict.
+    -- entailer. Exists v ls. entailer. unfold type_kalloc_token.
+    rewrite kalloc_token_sz_split. rewrite mem_mgr_split. entailer!.
+    ++ destruct ls.
+     left; split; auto. rewrite <- H10; auto.
+     right; split; auto. unfold not; intros. auto_contradict.
+     rewrite <- H11. unfold not; intros. auto_contradict.
+    ++ 
+ 
+    sep_apply data_at_memory_block. unfold offset_val. destruct original_freelist_pointer; auto_contradict. 
+    assert (Ptrofs.add i (Ptrofs.repr t_run_size) = Ptrofs.repr (Ptrofs.unsigned i + t_run_size)). {
+    rewrite Ptrofs.add_unsigned. rewrite Ptrofs.unsigned_repr; unfold t_run_size; simpl; try rep_lia. auto.
+    }
+    rewrite H15.
+    assert (i = Ptrofs.repr (Ptrofs.unsigned i)). { rewrite Ptrofs.repr_unsigned. auto. }
+    replace (i) with (Ptrofs.repr (Ptrofs.unsigned i)) at 1.
+    entailer!.
+    unfold malloc_compatible. 
+    rewrite <- memory_block_split.
+    **
+    rewrite <- H16 at 1. 
+    assert (t_run_size + (PGSIZE - t_run_size) = PGSIZE). { simpl. unfold PGSIZE; try rep_lia. }
+    rewrite H19. entailer!.
+    ** 
+    unfold t_run_size; simpl; try rep_lia.
+    **
+    unfold PGSIZE, t_run_size; simpl; try rep_lia.
+    ** simpl. split; try rep_lia. unfold PGSIZE in H4; try rep_lia.
+    + forward. entailer.
+    + forward. if_tac_auto_contradict. Intros next ls'.
+    Exists next ls'. 
+    entailer!.
+Qed.
+
+
+
+(*Lemma body_kalloc: semax_body KAFVprog KAFGprog f_kalloc (kalloc_spec (KAF_APD) t_run).
 Proof. start_function.
 rewrite mem_mgr_split. Intros. forward.
 forward_if (
@@ -69,5 +196,5 @@ forward_if (
 -forward. destruct (eq_dec original_freelist_pointer nullval) eqn:e1; auto_contradict. entailer.
 rewrite mem_mgr_split. entailer.
 - if_tac; forward.
-Qed.
+Qed.*)
 
